hfc/FFAMemoryHypCallWellFormedProof.v
@@ -32,14 +32,6 @@ Local Open Scope monad_scope.
 Local Open Scope string_scope.
 Require Import Coqlib sflib.
 
-
-Inductive terminate {E} {R} (it:itree E R) : Prop :=
-| TermRet
-    v
-    (RET: observe it = RetF v)
-| TermTau
-    (TAU: observe it = TauF it).
-
 (* From HafniumCore *)
 Require Import Lang.
 Require Import Values.
@@ -49,23 +41,11 @@ Import LangNotations.
 Local Open Scope expr_scope.
 Local Open Scope stmt_scope.
 
-Require Export FFAMemoryHypCallsState.
-
-Section WELLFORMED.
-  
-  (* basic invariants *) 
-  Definition well_formed (st: AbstractState) : Prop := True. 
-  
-  (* TODO: need to add  more state in here - e.g. register values defined in interfaces / 
-     permissions of each page entry 
-     described in the FF-A document *)
-
-End WELLFORMED.
+Require Export FFAMemoryHypCallState.
+Require Export FFAMemoryHypCall.
 
 Section WELLFORMEDLEMMA.
-
-  Context `{high_spec_context: HighSpecContext}.
-
+  
   (*
   Lemma ffa_mem_send_well_formed_preserve:
     forall (st: AbstractState) (share_func : FFA_FUNCTION_TYPE) (length address page_count: Z),
@@ -78,4 +58,20 @@ Section WELLFORMEDLEMMA.
    *)
   
 End WELLFORMEDLEMMA.
+
+
+Section WELLFORMEDPROOF.
+  
+  (*
+  Lemma ffa_mem_send_well_formed_preserve:
+    forall (st: AbstractState) (share_func : FFA_FUNCTION_TYPE) (length address page_count: Z),
+      well_formed st ->
+      match api_ffa_mem_send share_func length address page_count st with
+      | Ret (_, st') => well_formed st 
+      | _ => True
+      end.
+  Admitted.
+   *)
+  
+End WELLFORMEDPROOF.
 
