hfc/FFAMemoryHypCall.v
@@ -45,6 +45,8 @@ Require Import Lang.
 Require Import Values.
 Require Import Integers.
 Require Import Constant.
+Require Import Decision.
+
 Import LangNotations.
 Local Open Scope expr_scope.
 Local Open Scope stmt_scope.
@@ -53,3 +55,381 @@ Import Int64.
 
 Require Import Maps.
 Set Implicit Arguments.
+
+Require Export FFAMemoryHypCallState.
+
+(*************************************************************)
+(*         Auxiliary functions                               *)
+(*************************************************************)
+Section FFAAuxiliaryFunctions.
+  
+  (* Auxiliary functions *)
+  (*
+  static inline ffa_vm_id_t ffa_msg_send_sender(struct ffa_value args)
+         {
+	   return (args.arg1 >> 16) & 0xffff;
+         }
+   *)
+
+  Definition ffa_msg_send_sender (args: FFA_value_type) : Z :=
+    Z.land (Z.shiftr (ZMap.get 1 (args.(vals))) 16) 65535.
+
+
+  (*
+  static inline ffa_vm_id_t ffa_msg_send_receiver(struct ffa_value args)
+  {
+          return args.arg1 & 0xffff;
+  }
+   *)
+  Definition ffa_msg_receiver_sender (args: FFA_value_type) : Z :=
+    Z.land (ZMap.get 1 (args.(vals))) 65535.
+
+  
+  (*
+  static inline uint32_t ffa_msg_send_size(struct ffa_value args)
+  {
+          return args.arg3;
+  }
+   *)
+  Definition ffa_msg_send_size (args: FFA_value_type) : Z :=
+    ZMap.get 3 args.(vals).
+
+  (*
+  static inline uint32_t ffa_msg_send_attributes(struct ffa_value args)
+  {
+          return args.arg4;
+  }
+   *)
+  Definition ffa_msg_send_attributes (args: FFA_value_type) : Z :=
+    ZMap.get 4 args.(vals).
+
+  (*
+  static inline ffa_memory_handle_t ffa_assemble_handle(uint32_t a1, uint32_t a2)
+  {
+          return (uint64_t)a1 | (uint64_t)a2 << 32;
+  }
+   *)
+  Definition ffa_assemble_handle (a1 a2 : Z) : ffa_memory_handle_t :=
+    Z.lor a1 (Z.shiftl a2 32).
+  
+
+  (*
+  static inline ffa_memory_handle_t ffa_mem_success_handle(struct ffa_value args)
+  {
+          return ffa_assemble_handle(args.arg2, args.arg3);
+  }
+  *)
+  Definition ffa_mem_success_handle (args : FFA_value_type) : ffa_memory_handle_t :=
+    ffa_assemble_handle (ZMap.get 2 args.(vals)) (ZMap.get 3 args.(vals)).
+
+  (*
+  static inline struct ffa_value ffa_mem_success(ffa_memory_handle_t handle)
+  {
+          return (struct ffa_value){.func = FFA_SUCCESS_32,
+          			  .arg2 = (uint32_t)handle,
+          			  .arg3 = (uint32_t)(handle >> 32)};
+  }
+   *)
+
+  Definition ffa_mem_success (handle : ffa_memory_handle_t) : FFA_value_type :=
+    mkFFA_value_type (FFA_RESULT_CODE_IDENTIFIER FFA_SUCCESS)
+                     (ZMap.set 2 handle (ZMap.set 3 (Z.shiftr handle 32) (ZMap.init 0))).
+    
+
+  (*
+  static inline ffa_vm_id_t ffa_vm_id(struct ffa_value args)
+  {
+          return (args.arg1 >> 16) & 0xffff;
+  }
+   *)
+
+  Definition ffa_vm_id (args : FFA_value_type) : ffa_vm_id_t :=
+    Z.land (ZMap.get 1 (args.(vals))) 65535.
+    
+  
+  (*
+  static inline ffa_vcpu_index_t ffa_vcpu_index(struct ffa_value args)
+  {
+          return args.arg1 & 0xffff;
+  }
+   *)
+  Definition ffa_vcpu_index (args : FFA_value_type) : ffa_vcpu_index_t :=
+    Z.land (ZMap.get 1 (args.(vals))) 65535.
+    
+  (*
+  static inline uint64_t ffa_vm_vcpu(ffa_vm_id_t vm_id,
+          			   ffa_vcpu_index_t vcpu_index)
+  {
+          return ((uint32_t)vm_id << 16) | vcpu_index;
+  }
+   *)
+  Definition ffa_vm_vcpu (vm_id : ffa_vm_id_t) (vcpu_index : ffa_vcpu_index_t) : Z :=
+    Z.lor (Z.shiftl vm_id 16) vcpu_index.
+
+  (*
+  /**
+   * Clear memory region contents after unmapping it from the sender and before
+   * mapping it for any receiver.
+   */
+  #define FFA_MEMORY_REGION_FLAG_CLEAR 0x1
+   
+  /**
+   * Whether the hypervisor may time slice the memory sharing or retrieval
+   * operation.
+   */
+  #define FFA_MEMORY_REGION_FLAG_TIME_SLICE 0x2
+   
+  /**
+   * Whether the hypervisor should clear the memory region after the receiver
+   * relinquishes it or is aborted.
+   */
+  #define FFA_MEMORY_REGION_FLAG_CLEAR_RELINQUISH 0x4
+   
+  #define FFA_MEMORY_REGION_TRANSACTION_TYPE_MASK ((0x3U) << 3)
+  #define FFA_MEMORY_REGION_TRANSACTION_TYPE_UNSPECIFIED ((0x0U) << 3)
+  #define FFA_MEMORY_REGION_TRANSACTION_TYPE_SHARE ((0x1U) << 3)
+  #define FFA_MEMORY_REGION_TRANSACTION_TYPE_LEND ((0x2U) << 3)
+  #define FFA_MEMORY_REGION_TRANSACTION_TYPE_DONATE ((0x3U) << 3)
+   *)
+
+
+  Definition FFA_MEMORY_REGION_FLAG_CLEAR_Z := 1.
+  Definition FFA_MEMORY_REGION_FLAAG_TIME_SLICE_Z := 2.
+  Definition FFA_MEMORY_REGION_FLAG_CLEAR_RELINGQUISH_Z := 4.
+
+  Definition FFA_MEMORY_REGION_TRANSACTION_TYPE_MASK_Z := Z.shiftl 3 3.
+  Definition FFA_MEMORY_REGION_TRANSACTION_TYPE_UNSPECIFIED_Z := Z.shiftl 0 3.
+  Definition FFA_MEMORY_REGION_TRANSACTION_TYPE_SHARE_Z := Z.shiftl 1 3.
+  Definition FFA_MEMORY_REGION_TRANSACTION_TYPE_LEND_Z := Z.shiftl 2 3.
+  Definition FFA_MEMORY_REGION_TRANSACTION_TYPE_DONATE_Z := Z.shiftl 3 3.
+
+  (* TODO : need to do something with the following functions *) 
+  (*
+  /**
+   * Gets the `ffa_composite_memory_region` for the given receiver from an
+   * `ffa_memory_region`, or NULL if it is not valid.
+   */
+  static inline struct ffa_composite_memory_region *
+  ffa_memory_region_get_composite(struct ffa_memory_region *memory_region,
+          			uint32_t receiver_index)
+  {
+          uint32_t offset = memory_region->receivers[receiver_index]
+          			  .composite_memory_region_offset;
+   
+          if (offset == 0) {
+          	return NULL;
+          }
+   
+          return (struct ffa_composite_memory_region * )((uint8_t * )memory_region +
+          					      offset);
+  }
+   
+  static inline uint32_t ffa_mem_relinquish_init(
+          struct ffa_mem_relinquish *relinquish_request,
+          ffa_memory_handle_t handle, ffa_memory_region_flags_t flags,
+          ffa_vm_id_t sender)
+  {
+          relinquish_request->handle = handle;
+          relinquish_request->flags = flags;
+          relinquish_request->endpoint_count = 1;
+          relinquish_request->endpoints[0] = sender;
+          return sizeof(struct ffa_mem_relinquish) + sizeof(ffa_vm_id_t);
+  }
+  *)
+   
+End FFAAuxiliaryFunctions.
+
+
+Inductive updateStateE: Type -> Type :=
+| GetState : updateStateE AbstractState
+| SetState (st: AbstractState): updateStateE unit.
+ 
+Definition updateState_handler {E: Type -> Type}
+  : updateStateE ~> stateT AbstractState (itree E) :=
+  fun _ e st =>
+    match e with
+    | GetState => Ret (st, st)
+    | SetState st' => Ret (st', tt)
+    end.
+ 
+Notation HafniumEE := (CallExternalE +' updateStateE +' GlobalE +' MemoryE +' Event).
+ 
+Notation "'do' X <- A ;;; B" := (match A with Some X => B | None => triggerUB "None" end)
+  (at level 200, X ident, A at level 100, B at level 200)
+  : itree_monad_scope.
+ 
+Notation "'do' X , Y <- A ;;; B" := (match A with Some (X, Y) => B | None => triggerUB "None" end)
+  (at level 200, X ident, Y ident, A at level 100, B at level 200)
+  : itree_monad_scope.
+ 
+Notation "'do' X , Y , Z <- A ;;; B" := (match A with Some (X, Y, Z) => B | None => triggerUB "None" end)
+  (at level 200, X ident, Y ident, Z ident, A at level 100, B at level 200)
+  : itree_monad_scope.
+ 
+Notation " 'check' A ;;; B" := (if A then B else Ret None)
+  (at level 200, A at level 100, B at level 200)
+  : itree_monad_scope.
+ 
+Local Open Scope itree_monad_scope.
+
+Section FFAMemoryHypCall.
+
+  Context `{address_translation: AddressTranslation}.
+  Context `{hafnium_memory_management_context :
+              !HafniumMemoryManagementContext (address_translation := address_translation)}.
+  Context `{vm_context : VMContext}.
+  Context `{abstract_state_context: !AbstractStateContext
+                                     (hafnium_memory_management_context
+                                        := hafnium_memory_management_context)}.
+
+  (************************************************************************)
+  (*                 Context switching related parts                      *)
+  (************************************************************************)
+  (* most parts are related to save registers in "/src/arch/aarch64/hypervisor/exceptions.S"
+     We dramatically simplify them by saving and restoring FFA-related register values. 
+     In reality, we may need to reflect the entire register save and recovery in the file:
+     "save_volatile_to_vcpu", "save_register_access", "vcpu_switch", "vcpu_restore_all_and_run",
+     "vcpu_restore_lazy_and_run", "vcpu_restore_nonvolatile_and_run", and 
+     "vcpu_restore_volatile_and_run" in  "/src/arch/aarch64/hypervisor/exceptions.S". 
+
+     In addition to that, "handle_system_register_access" in "/src/arch/aarch64/hypervisor/handler.c"
+     also a function that handles register values when handling exceptions. 
+
+     How it works:
+     When an exception occurs, it first checks the exception value in the register ("vector_table_el2" 
+     in the file). Then, if the exception number is either "sync_lower_64" or "sync_lower_32", 
+     it calls "lower_sync_exception" defined in the same file. 
+     
+     Then, "lower_sync_exception" performs context switching and calls a C handler function to
+     service the exception.
+  *)  
+  Section FFAContextSwitching.
+
+    (* Save contexts *)
+    Definition save_regs_to_vcpu_spec  :
+      itree HafniumEE (unit) := 
+      st <- trigger GetState;;
+      (* check whether the current running entity is one of VMs *)
+      if decide (st.(cur_entity_id) <> hafnium_id) && in_dec zeq st.(cur_entity_id) vm_ids
+      then do vm_client <- ZTree.get st.(cur_entity_id) st.(vms_clients) ;;;
+           do vm_context <- ZTree.get st.(cur_entity_id) st.(hafnium_context).(vms_contexts) ;;;
+           do vcpu_regs <- ZTree.get vm_client.(client_cur_vcpu_id) vm_client.(client_vcpu_struct) ;;;
+           if decide (vm_context.(vcpu_num) = vm_client.(client_vcpu_num))    
+           then
+             let new_vcpu_id := vm_client.(client_cur_vcpu_id) in
+             let new_vm_context := 
+                 mkVM_struct new_vcpu_id (vm_context.(vcpu_num))
+                             (ZTree.set (new_vcpu_id) vcpu_regs vm_context.(vcpu_struct)) in
+             let new_vms_contexts :=
+                 ZTree.set st.(cur_entity_id) new_vm_context st.(hafnium_context).(vms_contexts) in
+             let new_st := st {cur_entity_id: hafnium_id}
+                              {hafnium_context/vms_contexts: new_vms_contexts} in 
+             trigger (SetState new_st)
+           else triggerUB "save_resg_to_vcpu_spec: inconsistency in vcpu number"
+      else triggerUB "save_resg_to_vcpu_spec: wrong cur entity id".
+
+    Definition save_regs_to_vcpu_call (args : list Lang.val) :=
+      match args with
+      | nil => save_regs_to_vcpu_spec
+      | _ => triggerUB "save_regs_to_vcpu_call: wrong arguments"
+      end.
+
+    (* Restore contexts and run.
+       It also contains choosing the next vm to run by using an abstract scheduler  
+     *)
+    Definition vcpu_restore_and_run_spec  :
+      itree HafniumEE (unit) := 
+      st <- trigger GetState;;
+      let next_vm_id := scheduler st in
+      (* check whether the current running entity is Hafnium *)
+      if decide (st.(cur_entity_id) = hafnium_id) && in_dec zeq next_vm_id vm_ids
+      then do vm_client <- ZTree.get next_vm_id st.(vms_clients) ;;;
+           do vm_context <- ZTree.get next_vm_id st.(hafnium_context).(vms_contexts) ;;;
+           do vcpu_regs <- ZTree.get vm_context.(cur_vcpu_id) vm_context.(vcpu_struct) ;;;
+           if decide (vm_context.(vcpu_num) = vm_client.(client_vcpu_num)) &&
+              decide (vm_context.(cur_vcpu_id) = vm_client.(client_cur_vcpu_id)) 
+           then
+             let new_vm_client :=
+                 mkVMClinet_struct (vm_client.(client_cur_vcpu_id)) (vm_client.(client_vcpu_num))
+                                   (ZTree.set (vm_client.(client_cur_vcpu_id))
+                                              vcpu_regs (vm_client.(client_vcpu_struct))) in
+             let new_vms_clients :=
+                 ZTree.set next_vm_id new_vm_client st.(vms_clients) in
+             let new_st := st {cur_entity_id: next_vm_id} {vms_clients: new_vms_clients} in 
+             trigger (SetState new_st)
+           else triggerUB "vcpu_restore_and_run__spec: inconsistency in vcpu number"
+      else triggerUB "vcpu_restore_and_run__spec: wrong cur entity id".
+
+    Definition vcpu_restore_and_run_call (args : list Lang.val) :=
+      match args with
+      | nil => vcpu_restore_and_run_spec
+      | _ => triggerUB "vcpu_restore_and_run_call: wrong arguments"
+      end.
+    
+  End FFAContextSwitching.
+
+  (************************************************************************)
+  (*                 FFA ABI for memory management                        *)
+  (************************************************************************)
+  (* All the following things are calls via "struct vcpu *sync_lower_exception(uintreg_t esr)" 
+     defined in "/src/arch/aarch64/hypervisor/handler.c". 
+
+     Depending on "uintreg_t ec = GET_ESR_EC(esr);", the exception case, the function calls
+     the proper handler. The main focus of our prototyping is when "EC_HVC", which are for 
+     hypervisor calls.
+     
+     "struct vcpu *hvc_handler(struct vcpu *vcpu)" is also a function that is defined in the same file.
+
+     For all cases that we consider in here, "(ffa_handler(&args, &next))" is a function 
+     that handles ffa related exceptions and return true.
+
+     "static bool ffa_handler(struct ffa_value *args, struct vcpu **next)" is also a function in the
+     the same file. Among all cases, cases they we are considering are as follows.
+
+     <<
+	case FFA_MEM_DONATE_32:
+	case FFA_MEM_LEND_32:
+	case FFA_MEM_SHARE_32:
+		*args = api_ffa_mem_send(func, args->arg1, args->arg2,
+					 ipa_init(args->arg3), args->arg4,
+					 current(), next);
+		return true;
+	case FFA_MEM_RETRIEVE_REQ_32:
+		*args = api_ffa_mem_retrieve_req(args->arg1, args->arg2,
+						 ipa_init(args->arg3),
+						 args->arg4, current());
+		return true;
+	case FFA_MEM_RELINQUISH_32:
+		*args = api_ffa_mem_relinquish(current());
+		return true;
+	case FFA_MEM_RECLAIM_32:
+		*args = api_ffa_mem_reclaim(
+			ffa_assemble_handle(args->arg1, args->arg2), args->arg3,
+			current());     
+    >>
+  *)
+  
+  (* Send is for three FFA ABIs, SHARE, DONATE, and LEND. *)
+  Section FFAMemoryHypCallSend.
+
+    
+    
+
+  End FFAMemoryHypCallSend.
+
+
+  Section FFAMemoryHypCallRetrieve.
+
+  End FFAMemoryHypCallRetrieve.
+
+
+  Section FFAMemoryHypCallRelingquish.
+
+  End FFAMemoryHypCallRelingquish.
+
+
+  Section FFAMemoryHypCallReclaim.
+
+  End FFAMemoryHypCallReclaim.
+  
+End FFAMemoryHypCall.
